Some new lemmas about environments
Also includes the definition of a new datatype, Vars, denoting non-empty
variable lists.

Env.v
@@ -1,4 +1,8 @@
-Require Import Var MSetList MSetProperties.
+(* TODO This file could probably do with a little more structure, consistent
+   naming and such. *)
+
+Require Import List1 MSetList MSetProperties Program.Basics TLC.LibTactics Var
+  Vars.
 
 Module S := MSetList.Make VarOrder.
 Module SF := MSetProperties.WPropertiesOn VarOrder S.
@@ -10,17 +14,66 @@ Notation env_add := S.add.
 Notation env_mem := S.In.
 Notation env_memb := SF.In_dec.
 Notation env_eq := S.Equal.
+Notation env_subset := S.Subset.
 Notation env_union := S.union.
 Notation env_singleton x := (env_add x env_empty).
 Notation env_fold := S.fold.
+Notation list_to_env := SF.of_list.
+
+Lemma env_mem_spec_subset :
+  forall x e e',
+  env_subset e e' ->
+  env_mem x e ->
+  env_mem x e'.
+Proof. intros. eapply SF.in_subset; eauto. Qed.
 
 Definition env_add_all (xs : list Var) (ys : Env) : Env :=
   fold_left (fun x y => env_add y x) xs ys.
+Definition env_subset_equal :
+  forall XS YS,
+  env_eq XS YS ->
+  env_subset XS YS
+  := SF.subset_equal.
 
 Definition env_add_assoc :
   forall XS X Y,
   env_eq (env_add X (env_add Y XS)) (env_add Y (env_add X XS))
   := SF.add_add.
+
+Instance env_add_m_subset (x : Var) : Proper (env_subset ==> env_subset) (env_add x).
+Proof. solve_proper. Qed.
+
+Definition env_union_list (xs : Env) (ys : list Var) : Env :=
+  fold_left (flip env_add) ys xs.
+
+Lemma env_union_list_neutral :
+  forall xs,
+  env_union_list xs nil = xs.
+Proof. auto. Qed.
+
+Definition env_union_vars (xs : Env) (ys : Vars) : Env :=
+  fold_left1 (fun x y => env_add y x) ys xs.
+
+Instance env_union_vars_m_subset :
+  Proper (env_subset ==> eq ==> env_subset) env_union_vars.
+Proof.
+  unfold Proper. unfold respectful. introv Hsub Heq. subst.
+  rename y0 into xs. gen x y. induction xs using list1_ind'; introv Hsub.
+    unfold env_union_vars. simpl. rewrite Hsub. reflexivity.
+
+    unfold env_union_vars in *. unfold cons1. destruct xs as [xs HxsNE].
+    simpl in *. apply IHxs. rewrite Hsub. reflexivity.
+Qed.
+
+Instance env_union_vars_m_env_eq :
+  Proper (env_eq ==> eq ==> env_eq) env_union_vars.
+Proof.
+  unfold Proper. unfold respectful. intros xs ys Hxsys xs' ys' Hxs'ys'.
+  subst. unfold env_union_vars. gen ys xs. destruct ys' as [ys' Hys'nonempty].
+
+  unfold fold_left1. simpl. clear Hys'nonempty. induction ys'; auto.
+  introv Hxsys. simpl in *. apply IHys'. rewrite Hxsys. reflexivity.
+Qed.
 
 Lemma env_add_twice :
   forall X XS,
@@ -53,7 +106,7 @@ Hint Resolve env_mem_empty : env.
 Lemma env_eq_spec :
   forall e e',
   env_eq e e' <-> (forall x, env_mem x e <-> env_mem x e').
-Proof with auto. intros; split; intros H; auto. Qed.
+Proof. intros; split; intros H; auto. Qed.
 
 Definition env_eq_refl :
   forall e,
@@ -114,3 +167,46 @@ Lemma env_union_assoc :
   forall e e' e'',
   env_eq (env_union (env_union e e') e'') (env_union e (env_union e' e'')).
 Proof. auto with set. Qed.
+
+Lemma env_subset_add :
+  forall XS X,
+  env_subset XS (env_add X XS).
+Proof. intros. rewrite env_add_union_singleton2. apply SF.union_subset_1. Qed.
+
+Definition env_subset_union1 :
+  forall e e',
+  env_subset e (env_union e e')
+  := SF.union_subset_1.
+
+Definition env_subset_union2 :
+  forall e e',
+  env_subset e' (env_union e e')
+  := SF.union_subset_2.
+
+Lemma env_union_vars_spec :
+  forall xs ys,
+  env_eq (env_union_vars xs ys) (env_union xs (list_to_env ys)).
+Proof.
+  unfold SF.of_list. unfold env_union_vars. unfold fold_left1. intros. gen xs.
+  induction ys using list1_ind'; intros.
+    simpl. rewrite env_add_union_singleton2. reflexivity.
+
+    destruct ys as [ys HysNE]. simpl in *. rewrite IHys.
+    rewrite <- env_add_union1. rewrite env_add_union2. reflexivity.
+Qed.
+
+Lemma env_union_list_spec :
+  forall xs ys,
+  env_eq (env_union_list xs ys) (env_union xs (list_to_env ys)).
+Proof.
+  unfold SF.of_list. unfold env_union_list. unfold flip. intros. gen xs.
+  induction ys; intros.
+    simpl. rewrite env_union_neutral. reflexivity.
+    simpl in *. rewrite IHys. rewrite <- env_add_union2.
+    rewrite env_add_union1. reflexivity.
+Qed.
+
+Lemma list_to_env_cons :
+  forall x xs,
+  env_eq (list_to_env (x :: xs)) (env_add x (list_to_env xs)).
+Proof. intros. unfold SF.of_list. simpl. reflexivity. Qed.
