Vars.v
@@ -1,0 +1,7 @@
+Require Import List1 Var.
+
+Notation Vars := (list1 Var).
+
+Definition In_Vars_dec := In1_dec eq_var_dec.
+
+Definition vars_eq := eq (A := Vars).
